\section{Notations, basic terminology}

In this first section we want to define the elementary terminology that is
used throughout the whole book. We use the usual notions
\begin{eqnarray*}
& & \mathbb{N} = \{ 0, 1, 2, \ldots \}\mbox{ for the natural numbers} \\
& & \mathbb{Z} = \{ \ldots, -2, -1, 0, 1, 2, \ldots \}\mbox{ for the integer
numbers} \\
& & \mathbb{Q} = \{ \frac{a}{b} \mid a,b \in \mathbb{Z}, b \neq 0 \}\mbox{ for
the rational numbers}
\end{eqnarray*}

For the operations on sets we use $\cup$ for the union and $\cap$ for the
intersection. Also $A \subset B$, $a \in A$, $a \not\in A$, $\bar{A}$, $A - B$,
$A \times B$ and $\emptyset$ have their usual meaning.

For the power set of a set $A$ we write $2^A$ or $Pot(A)$. $Card(A)$ denotes the
cardinality of $A$.

Logical implication is denoted by $\Rightarrow$.

{\bf Mappings} are denoted as $f : A \rightarrow B$, in which case $f$ is a
total mapping. We write $Q(f) = A, Z(f) = B$. 

\transrem{$Q$ stands for German ''Quelle'' (source) and $Z$ for ''Ziel''
(target).}

If $f: A \rightarrow B,\ g : B \rightarrow C$ are mappings, then $f \circ g : A
\rightarrow C$ is the {\bf composition} which one gets by applying
\boldmath $f$ {\bf first and then} $g$ \unboldmath: 
\[(f \circ g)(a) = g(f(a))\]
If $f:A \rightarrow B$ and $C \subset A$, then $f(C) = \{ f(c) \mid c \in C \}$.

\transrem{Note that this is the other way round than the usual
definition of function composition but makes perfect sense here in the category theoretic
framework.}

A subset $R \subset A \times B$ is called a {\bf relation} between $A$ and $B$.
\[R_f = \{ (a,b) \mid b = f(a) \} \subset A \times B\] 
is the relation {\bf induced by} the mapping f or also the {\bf graph} of $f$.

Let $f : A \rightarrow B$ be a mapping, $A_1 \subset A$ and $g : A_1 \rightarrow
B$ a mapping. 

$f$ is called the {\bf continuation} of $g$ if $f(a_1) = g(a_1),
a_1 \in A_1$. In this case we also write $f \mid _{A_1} = g$, in words: $f$
{\bf restricted to} $A_1$.

A {\bf semi-group} consists of a set $M$ and an associative operation on that
set, usually denoted as a multiplication. If a semi-group is commutative, we
also use ''$+$'' instead of ''$\cdot$''.

A semi-group is a \index{{\bf monoid}} if $M$ contains a neutral element. We
often denote it with $1_M$ or shortly $1$. In the commutative case we often write $0$
instead of $1$.

For $A,B \subset M$ we denote by 
\[ A \cdot B = \{ a \cdot b \mid a \in A, b \in B \}\]
the {\bf complex product} of $A$ and $B$.

$A \subset M$ is a {\bf submonoid} of $M$ if $1_M \in A$ and $A$ is closed under
the operation of $M$.

For a set $A$, the set $A^*$ defined as follows, is the smallest submonoid of
$M$ containing $A$. 

More specific,
\[ A^* = \bigcap_{U \in M(A)} U	\]
where 
\[ M(A) = \{ U \subset M \mid U \mbox{ is a submonoid of } M, A \subset U \} \]

It is easy to see that 
\[ A^* = \bigcup_{n \geq 0} A^n \mbox{ with }A^0 = \{ 1 \}\mbox{ and }A^{n+1}
= A^n \cdot A \]

In the same sense the notion $A^+ = A^* - \{1\}$ is defined for semi-groups. $A$
is called the {\bf generating system} of $A^*$ and $A^+$ resp.

A special meaning for us is assigned to the set of {\em words (strings)} over a
fixed alphabet $A$. We understand as words the finite sequences of elements from
the alphabet $A$, for example $(a,b,d,a,c)$ over the alphabet $A = \{ a,b,c,d
\}$.

We define
\[ WORD(A) := \{\epsilon\} \cup A \cup (A \times A) \cup (A \times A \times A)
\cup \ldots \]
as the {\bf set of words (strings)} over $A$. 

The symbol $\epsilon$ denotes the {\bf empty word} over $A$, that is $A^0 =
\{\epsilon\}$.

If $v, w \in WORD(A)$ then $v \cdot w$ is the word which you get by
concatenating $v$ and $w$, formally:
\[ v = (a_1,\ldots, a_k),\ w = (a_{k+1}, \ldots, a_n) \Rightarrow v \cdot
w = (a_1, \ldots, a_n) \]

With this operation, $WORD(A)$ becomes a monoid which is usually also denoted
with $A^*$.

This naming is slightly inconsistent because for the first definition of
the $*$-operator it holds $(A^*)^* = A^*$ but for the second usage of the
$*$-operator it holds $(A*)^* \neq A^*$.

The following example should clarify this fact: 

Let $A = \{a,b,c\}$ and let $(a,b,a)$ and $(b,a) \in A^*$.
\[(a,b,a)\cdot(b,a) = (a,b,a,b,a) \in A^*,\mbox{ but} \]
\[((a,b,a),(b,a)) \in (A^*)^*\mbox{ but }\notin A^* \]

Instead of $(a)$ we just write $a$. In this sense it holds $A \subset A^*$. This
also holds in the sense of the first definition of $A^*$.

If $w = (w_1, \ldots, w_n)$ we call $|w| := n$ the {\bf length} of $w$.
Obviously 
\[|w \cdot v| = |w| + |v|\mbox{ and }|\epsilon| = 0\]

The {\bf mirror word} of a word $w = (w_1,\ldots,w_n)$ is the word
$w^R = (w_n,\ldots,w_1)$. It holds:
\[ (w \cdot v)^R = v^R \cdot w^R \text{ and }\epsilon^R = \epsilon \]

In $A^*$ the {\bf cancellation rules} hold, i.e.
\begin{enumerate}
  \item $w \cdot x = w \cdot y \Rightarrow x = y$
  \item $x \cdot w = y \cdot w \Rightarrow x = y$
\end{enumerate}

We define {\bf left} and {\bf right quotient}:
\[ X^{-1} \cdot Y = \{ w \mid \exists x \in X,\ y \in Y\mbox{ with }x \cdot w
= y \} \] 
and 
\[ X \cdot Y^{-1} = \{ w \mid \exists x \in X,\ y \in Y\mbox{ with } w \cdot y
= x \} \]

Because of the cancellation rules it holds:
\[ \{w\}^{-1} \cdot \{v\}\mbox{ and } \{ w \}^{-1} \cdot \{ v \}\mbox{ are
either empty or contain a single element.} \]

If $\{ w \}^{-1} \cdot \{ v \}$ is not empty, we call $w$ a {\bf prefix} of $v$,
if $\{ w \} \cdot \{ v \}^{-1} \not= \emptyset$, we call $v$ a {\bf suffix} of
$w$.

In the future we will always write just $w$ instead of $\{ w \}$ and also $w$
{\bf is prefix of} $v$, if $w^{-1} \cdot v \not= \emptyset$.
